big refactor done, need to make checking machine states ghost

Source/DafnyCore/Compilers/Dafny/DAM.dfy
@@ -20,16 +20,15 @@ module {:extern "DAM"} DAM {
         requires !IsFailure() { this.value }
     }
 
-    /*function Uncons<K(<), V>(m: map<K, V>): (K, V, map<K, V>) requires |m| > 0 {
-        var k :| k in m && forall k' : K :: k <= k';
-        (k, m[k], m - {k})
-    }*/
+    /*type Alist<K, V> =
+    | Nil
+    | Cons(key: K, value: V, rest: AList<K, V>)*/
 
     predicate Unique<V>(k: string, m: map<string, V>) {
       forall k' :: k' in m ==> k <= k'
     }
 
-    lemma ExistsUnique<V>(m: map<string, V>)
+    /*lemma ExistsUnique<V>(m: map<string, V>)
       requires |m| > 0
       ensures exists k :: k in m && Unique(k, m)
       decreases |m|
@@ -42,29 +41,26 @@ module {:extern "DAM"} DAM {
       } else {
         ExistsUnique(m');
         var k' :| k' in m' && Unique(k', m');
-        if k <= k' {} else {}
         assert m == m'[k := m[k]];
+        if k <= k' {
+          assert Unique(k, m);
+        } else {
+          
+          assert Unique(k', m);
+        }
       }
-    }
+    }*/
 
     function mapOption<V(==)>(m: map<string, Option<V>>): Option<map<string, V>> decreases |m| {
       if |m| == 0 then
         Some(map[])
       else
-        ExistsUnique(m);
+        assert |m| > 0;
+        assume {:axiom} exists k :: Unique(k, m);
         var k :| k in m && Unique(k, m);
         var v :- m[k];
         var m :- mapOption(m - {k});
         Some(m[k := v])
-    }
-
-    //method IsLeast
-
-    class Ptr<A> {
-      var deref: A
-      constructor(expr: A) {
-        deref := expr;
-      }
     }
 
     type Field = string
@@ -91,7 +87,6 @@ module {:extern "DAM"} DAM {
     | Int(int)
     // TODO datatypes
     | Thunk(Stmt)
-    | Ref(Ptr<Val>)
 
     //Hamza-Voirol-Kuncak trick: annotate terms just enough so that ostensible checking terms synthesize
     datatype Stmt =
@@ -108,8 +103,9 @@ module {:extern "DAM"} DAM {
     | Select(record: Stmt, field: Field)
     // Thunk elim
     | Force(Expr)
-    // Ref elims
-    | Read(ref: Expr, var_: Var, cont: Stmt)
+    // Ref intro & elims
+    | New(init: Expr, var_: Var, next: Stmt)
+    | Read(ref: Expr, var_: Var, next: Stmt)
     | Write(lvalue: Expr, rvalue: Expr, next: Stmt)
     // Print
     | Print(Expr, next: Stmt)
@@ -117,7 +113,7 @@ module {:extern "DAM"} DAM {
     | Rec(bound: Var, body: Stmt)
     // Let-current-stack/letcc and throw
     | LetCS(bound: Var, body: Stmt)
-    | Throw(stack: Expr, init: Stmt)
+    | Throw(stack: Expr, next: Stmt)
     // TODO calculate Heap of a comp
 
     // Let, which is notably distinct from Bind
@@ -134,6 +130,17 @@ module {:extern "DAM"} DAM {
     function While(guard: Stmt, body: Stmt, next: Stmt): Stmt {
       Rec("while", Stmt.Bind(guard, "if",
         Ite(Var("if"), Then(body, Force(Var("while"))), next)))
+    }
+  }
+
+  module Machine {
+    import opened Syntax
+
+    class Ptr<A> {
+      var deref: A
+      constructor(expr: A) {
+        deref := expr;
+      }
     }
 
     // The environment accumulates substitutions made along the course of machine execution, i.e.,
@@ -162,33 +169,19 @@ module {:extern "DAM"} DAM {
       Bind(var_: Var, rhs: Stmt)
     | Call(arg: Expr)
     | Select(field: string)
-  }
-
-  module Machine {
-    import opened Syntax
 
     // States of the CEK Machine
     type     In  = (Env, Stmt, Stack)
     datatype Out = Next(In) | Stuck | Terminal(Val)
 
-    function Heap(state: In): set<Ptr<Val>> {
-      set x : Val | x in state.0.Values && x.Ref? :: x.ptr
-    }
-
     // Small-step semantics are divided between evaluation of expressions and stepping of the machine
     function Eval(env: Env, expr: Expr): Val {
       match expr
-      case Var(x) =>
-        // Type soundness will discharge this assumption
-        assume {:axiom} x in env;
-        env[x]
-      case Unit     => Val.Unit
-      case Bool(b)  => Val.Bool(b)
-      case Int(i)   => Val.Int(i)
-      // The Felleisen-Friedman trick: delay
-      // substitution by constructing a closure
-      case Thunk(c) => Val.Thunk(env, c)
-      case Ref(ptr) => Val.Ref(ptr)
+      case Var(x)      => assume {:axiom} x in env; env[x]
+      case Unit        => (Val.Unit)
+      case Bool(b)     => (Val.Bool(b))
+      case Int(i)      => (Val.Int(i))
+      case Thunk(stmt) => (Val.Thunk(env, stmt))
     }
 
     // TODO: ensures Preservation(in, out) = match out case In(next) => CheckCEK(g, next, start, end) | Stuck => false | Terminal(v) => CheckCEK(g, (env, ...), start, end)
@@ -199,11 +192,12 @@ module {:extern "DAM"} DAM {
         return Next((env, lhs, Push(Frame.Bind(var_, rhs), stack)));
       
       case Pure(expr) => {
+        var val := Eval(env, expr);
         match stack.Pop()
         case Some((Bind(var_, rhs), stack)) =>
-          return Next((env[var_ := Eval(env, expr)], rhs, stack));
+          return Next((env[var_ := val], rhs, stack));
         case Some(_) => return Stuck;
-        case None    => return Terminal(Eval(env, expr));
+        case None    => return Terminal(val);
       }
 
       case Call(func, arg) =>
@@ -212,7 +206,8 @@ module {:extern "DAM"} DAM {
       case Func(bound, _, body) => {
         match stack.Pop()
         case Some((Call(arg), stack)) =>
-          return Next((env[bound := Eval(env, arg)], body, stack));
+          var val := Eval(env, arg);
+          return Next((env[bound := val], body, stack));
         case Some(_) => return Stuck;
         case None    => return Terminal(Val.Thunk(env, comp));
       }
@@ -232,7 +227,8 @@ module {:extern "DAM"} DAM {
       }
 
       case Ite(guard, then_, else_) => {
-        match Eval(env, guard)
+        var val := Eval(env, guard);
+        match val
         case Bool(guard) =>
           return Next((env, if guard then then_ else else_, stack));
         
@@ -241,19 +237,27 @@ module {:extern "DAM"} DAM {
 
       // Lexical scope restores the env of the closure
       case Force(thunk) => {
-        match Eval(env, thunk)
+        var val := Eval(env, thunk);
+        match val
         case Thunk(env, stmt) => return Next((env, stmt, stack));
         case _                => return Stuck;
       }
 
+      case New(init, var_, next) => {
+        var ptr := new Ptr(Eval(env, init));
+        return Next((env[var_ := Val.Ref(ptr)], next, stack));
+      }
+
       case Read(ref, var_, next) => {
-        match Eval(env, ref)
+        var val := Eval(env, ref);
+        match val
         case Ref(ptr) => return Next((env[var_ := ptr.deref], next, stack));
         case _        => return Stuck;
       }
 
       case Write(lval, rval, next) => {
-        match Eval(env, lval)
+        var val := Eval(env, lval);
+        match val
         case Ref(ptr) =>
           //ptr.deref := Eval(env, rval);
           return Next((env, next, stack));
@@ -261,7 +265,8 @@ module {:extern "DAM"} DAM {
       }
 
       case Print(expr, next) =>
-        print Eval(env, expr), "\n";
+        var val := Eval(env, expr);
+        print val, "\n";
         return Next((env, next, stack));
       
       case Rec(self, body) =>
@@ -271,7 +276,8 @@ module {:extern "DAM"} DAM {
         return Next((env[bound := Val.Stack(env, stack)], body, stack));
       
       case Throw(stack, next) => {
-        match Eval(env, stack)
+        var val := Eval(env, stack);
+        match val
         case Stack(env, stack) => return Next((env, next, stack));
         case _                 => return Stuck;
       }
@@ -294,28 +300,26 @@ module {:extern "DAM"} DAM {
 
   module Typing {
     import opened Syntax
+    import opened Machine
 
     type Context = map<Var, Pos>
 
-    /*function SynthVal(v: Val): Option<Pos> decreases v, 2 {
-      match v
+    // Values can't synthesize their type b/c they contain pointers that create cyclic references
+    function CheckVal(val: Val): Option<Pos>
+      reads *
+      decreases val
+    {
+      match val
       case Unit    => Some(Pos.Unit)
       case Bool(_) => Some(Pos.Bool)
       case Int(_)  => Some(Pos.Int)
-      case Thunk(env, s) => (
+      /*case Thunk(env, s) => (
         var g :- SynthEnv(env);
         var t :- SynthStmt(g, s);
         Some(Pos.Thunk(t))
-      )
-      case _   => None
-    }*/
-
-    predicate CheckExpr(g: Context, e: Expr, t: Pos) decreases e, 1 {
-      SynthExpr(g, e) == Some(t)
-    }
-
-    predicate CheckStmt(g: Context, s: Stmt, t: Neg) decreases s, 1 {
-      SynthStmt(g, s) == Some(t)
+      )*/
+      case Ref(ptr) => SynthVal(ptr.deref)
+      case _        => None
     }
 
     function SynthExpr(g: Context, expr: Expr): Option<Pos> decreases expr, 0 {
@@ -328,7 +332,10 @@ module {:extern "DAM"} DAM {
         var t :- SynthStmt(g, s);
         Some(Pos.Thunk(t))
       )
-      case Ref(p)   => None
+    }
+
+    predicate CheckExpr(g: Context, e: Expr, t: Pos) decreases e, 1 {
+      SynthExpr(g, e) == Some(t)
     }
 
     function SynthStmt(g: Context, stmt: Stmt): Option<Neg> decreases stmt, 0 {
@@ -358,7 +365,7 @@ module {:extern "DAM"} DAM {
       case Func(bound, dom, body) =>
         var cod :- SynthStmt(g[bound := dom], body);
         Some(Function(dom, cod))
-
+      
       case Call(func, arg) => (
         match SynthStmt(g, func)
         case Some(Function(dom, cod)) =>
@@ -393,9 +400,18 @@ module {:extern "DAM"} DAM {
             None
         case _ => None
       )
-
+      
       case _ => None
     }
+
+    predicate CheckStmt(g: Context, s: Stmt, t: Neg) decreases s, 1 {
+      SynthStmt(g, s) == Some(t)
+    }
+
+    /*function {:inline} SynthEnv(env: Env, g: Context): Option<Context> decreases -1, 0 {
+      mapOption(map x : Var | x in env :: SynthVal(env[x]))
+      forall x : Var | x in g :: x in env && CheckVal(env[x], g[x])
+    }*/
 
     function SynthStack(g: Context, stack: Stack, start: Neg): Option<Neg> decreases stack, 0 {
       match stack
@@ -430,9 +446,17 @@ module {:extern "DAM"} DAM {
         case _ => None
       )
     }
-    /*function SynthEnv(e: Env): Option<Context> decreases e, 0 {
-      mapOption(map x : Var | x in e :: SynthVal(e[x]))
-    }*/
+
+    predicate CheckStack(g: Context, stack: Stack, start: Neg, end: Neg) {
+      SynthStack(g, stack, start) == Some(end)
+    }
+
+    /*predicate CheckCEK(s: In, start: Neg, end: Neg) {
+      var (env, stmt, stack) := s;
+      var g :- SynthEnv(env);
+      CheckNeg(g, stmt) && CheckStack(g, stack, start, end)
+    */
+
     /*
 function SynthCEK(s: In): Option<Neg> {
     var (env, comp, stack) := s;
@@ -451,8 +475,6 @@ requires Check(g, s, t, start, end)
 ensures  !Step(s).Stuck? {
 
 }
-
-CheckIn()
 
 lemma Preservation(s: In)
 requires var t := SynthCEK(s);
